Fix bug in semantics: a configuration step consists of one or more thread steps

src/lang/Configuration.v
@@ -119,9 +119,19 @@ Module Configuration.
       e tid c1 lang st1 lc1 e2 st3 lc3 sc3 memory3
       (TID: IdentMap.find tid c1.(threads) = Some (existT _ lang st1, lc1))
       (STEPS: rtc (@Thread.tau_step _) (Thread.mk _ st1 lc1 c1.(sc) c1.(memory)) e2)
-      (STEP: Thread.opt_step e e2 (Thread.mk _ st3 lc3 sc3 memory3))
+      (STEP: Thread.step e e2 (Thread.mk _ st3 lc3 sc3 memory3))
       (CONSISTENT: Thread.consistent (Thread.mk lang st3 lc3 sc3 memory3)):
       step (ThreadEvent.get_event e) tid c1 (mk (IdentMap.add tid (existT _ _ st3, lc3) c1.(threads)) sc3 memory3)
+  .
+
+  Inductive opt_step: forall (e:option Event.t) (tid:Ident.t) (c1 c2:t), Prop :=
+  | step_none
+      tid c:
+      opt_step None tid c c
+  | step_some
+      e tid c1 c2
+      (STEP: step e tid c1 c2):
+      opt_step e tid c1 c2
   .
 
   Inductive tau_step (c1 c2:t): Prop :=
@@ -161,24 +171,24 @@ Module Configuration.
     inv WF1. inv WF. inv STEP. s.
     exploit THREADS; ss; eauto. i.
     exploit Thread.rtc_step_future; eauto. s. i. des.
-    exploit Thread.opt_step_future; eauto. s. i. des.
+    exploit Thread.step_future; eauto. s. i. des.
     splits; [| |by etrans; eauto|by etrans; eauto].
     - econs; ss. econs.
       + i. simplify.
         * congr.
         * exploit THREADS; try apply TH1; eauto. i. des.
           exploit Thread.rtc_step_disjoint; eauto. i. des.
-          exploit Thread.opt_step_disjoint; eauto. s. i. des.
+          exploit Thread.step_disjoint; eauto. s. i. des.
           symmetry. auto.
         * exploit THREADS; try apply TH2; eauto. i. des.
           exploit Thread.rtc_step_disjoint; eauto. i. des.
-          exploit Thread.opt_step_disjoint; eauto. i. des.
+          exploit Thread.step_disjoint; eauto. i. des.
           auto.
         * eapply DISJOINT; [|eauto|eauto]. auto.
       + i. simplify.
         exploit THREADS; try apply TH; eauto. i.
         exploit Thread.rtc_step_disjoint; eauto. i. des.
-        exploit Thread.opt_step_disjoint; eauto. s. i. des.
+        exploit Thread.step_disjoint; eauto. s. i. des.
         auto.
     - ii. simplify; eauto.
       eapply CONSISTENT1; eauto.
@@ -204,7 +214,7 @@ Module Configuration.
     { apply WF1. }
     { apply WF1. }
     s. i. des.
-    exploit Thread.opt_step_future; eauto. s. i. des.
+    exploit Thread.step_future; eauto. s. i. des.
     splits.
     - econs; s; ii; simplify.
       + inv DISJOINT. eapply THREAD; eauto.
@@ -216,7 +226,7 @@ Module Configuration.
         { eapply DISJOINT; eauto. }
         { eapply WF; eauto. }
         i. des.
-        exploit Thread.opt_step_disjoint; eauto. s. i. des.
+        exploit Thread.step_disjoint; eauto. s. i. des.
         auto.
       + inv DISJOINT. eapply MEMORY; eauto.
     - econs; s; eauto.
@@ -230,7 +240,7 @@ Module Configuration.
           { eapply DISJOINT; eauto. }
           { eapply WF; eauto. }
           i. des.
-          exploit Thread.opt_step_disjoint; eauto. s. i. des.
+          exploit Thread.step_disjoint; eauto. s. i. des.
           splits; ss.
     - ii. ss.
       exploit Thread.rtc_step_disjoint; eauto.
@@ -240,10 +250,42 @@ Module Configuration.
       { eapply DISJOINT; eauto. }
       { eapply WF; eauto. }
       i. des.
-      exploit Thread.opt_step_disjoint; eauto. s. i. des.
+      exploit Thread.step_disjoint; eauto. s. i. des.
       eapply CONSISTENT; eauto.
       + s. etrans; eauto. etrans; eauto.
       + s. etrans; eauto. etrans; eauto.
+  Qed.
+
+  Lemma opt_step_future
+        e tid c1 c2
+        (STEP: opt_step e tid c1 c2)
+        (WF1: wf c1)
+        (CONSISTENT1: consistent c1):
+    <<WF2: wf c2>> /\
+    <<CONSISTENT2: consistent c2>> /\
+    <<SC_FUTURE: TimeMap.le c1.(sc) c2.(sc)>> /\
+    <<MEM_FUTURE: Memory.future c1.(memory) c2.(memory)>>.
+  Proof.
+    inv STEP.
+    - splits; auto; refl.
+    - eapply step_future; eauto.
+  Qed.
+
+  Lemma opt_step_disjoint
+        e tid c1 c2 ths
+        (STEP: opt_step e tid c1 c2)
+        (DISJOINT: Threads.disjoint c1.(threads) ths)
+        (WF1: wf c1)
+        (CONSISTENT1: consistent c1)
+        (WF: wf (mk ths c1.(sc) c1.(memory)))
+        (CONSISTENT: consistent (mk ths c1.(sc) c1.(memory))):
+      <<DISJOINT: Threads.disjoint c2.(threads) ths>> /\
+      <<WF: wf (mk ths c2.(sc) c2.(memory))>> /\
+      <<CONSISTENT: consistent (mk ths c2.(sc) c2.(memory))>>.
+  Proof.
+    inv STEP.
+    - splits; auto; refl.
+    - eapply step_disjoint; eauto.
   Qed.
 
   Lemma rtc_step_future
